Weidenbach_Book/IsaSAT/IsaSAT_Setup.thy
@@ -1270,5 +1270,87 @@ definition heuristic_reluctant_untrigger_st :: \<open>twl_st_wl_heur \<Rightarro
   vdom, avdom, lcount, opts, old_arena).
   (M', N', D', j, W', vm, clvls, cach, lbd, outl, stats, heuristic_reluctant_untrigger heur,
        vdom, avdom, lcount, opts, old_arena))\<close>
+lemma twl_st_heur''D_twl_st_heurD:
+  assumes H: \<open>(\<And>\<D> r. f \<in> twl_st_heur'' \<D> r lcount \<rightarrow>\<^sub>f \<langle>twl_st_heur'' \<D> r lcount\<rangle> nres_rel)\<close>
+  shows \<open>f \<in> {(S, T). (S, T) \<in> twl_st_heur \<and> get_learned_count S = lcount} \<rightarrow>\<^sub>f
+        \<langle>{(S, T). (S, T) \<in> twl_st_heur \<and> get_learned_count S = lcount}\<rangle> nres_rel\<close>  (is \<open>_ \<in> ?A B\<close>)
+proof -
+  obtain f1 f2 where f: \<open>f = (f1, f2)\<close>
+    by (cases f) auto
+  show ?thesis
+    unfolding f
+    apply (simp only: fref_def twl_st_heur'_def nres_rel_def in_pair_collect_simp)
+    apply (intro conjI impI allI)
+    subgoal for x y
+      using assms[of \<open>dom_m (get_clauses_wl y)\<close>  \<open>length (get_clauses_wl_heur x)\<close>,
+        unfolded twl_st_heur'_def nres_rel_def in_pair_collect_simp f,
+        rule_format] unfolding f
+      apply (simp only: fref_def twl_st_heur'_def nres_rel_def in_pair_collect_simp)
+      apply (drule spec[of _ x])
+      apply (drule spec[of _ y])
+      apply simp
+      apply (rule "weaken_\<Down>'"[of _ \<open>twl_st_heur'' (dom_m (get_clauses_wl y))
+        (length (get_clauses_wl_heur x)) lcount\<close>])
+      apply (fastforce simp: twl_st_heur'_def)+
+      done
+    done
+qed
+
+
+lemma twl_st_heur'''D_twl_st_heurD:
+  assumes H: \<open>(\<And>r. f \<in> twl_st_heur''' r \<rightarrow>\<^sub>f \<langle>twl_st_heur''' r\<rangle> nres_rel)\<close>
+  shows \<open>f \<in> twl_st_heur \<rightarrow>\<^sub>f \<langle>twl_st_heur\<rangle> nres_rel\<close>  (is \<open>_ \<in> ?A B\<close>)
+proof -
+  obtain f1 f2 where f: \<open>f = (f1, f2)\<close>
+    by (cases f) auto
+  show ?thesis
+    unfolding f
+    apply (simp only: fref_def twl_st_heur'_def nres_rel_def in_pair_collect_simp)
+    apply (intro conjI impI allI)
+    subgoal for x y
+      using assms[of \<open>length (get_clauses_wl_heur x)\<close>,
+        unfolded twl_st_heur'_def nres_rel_def in_pair_collect_simp f,
+        rule_format] unfolding f
+      apply (simp only: fref_def twl_st_heur'_def nres_rel_def in_pair_collect_simp)
+      apply (drule spec[of _ x])
+      apply (drule spec[of _ y])
+      apply simp
+      apply (rule "weaken_\<Down>'"[of _ \<open>twl_st_heur''' (length (get_clauses_wl_heur x))\<close>])
+      apply (fastforce simp: twl_st_heur'_def)+
+      done
+    done
+qed
+
+
+lemma twl_st_heur'''D_twl_st_heurD_prod:
+  assumes H: \<open>(\<And>r. f \<in> twl_st_heur''' r \<rightarrow>\<^sub>f \<langle>A \<times>\<^sub>r twl_st_heur''' r\<rangle> nres_rel)\<close>
+  shows \<open>f \<in> twl_st_heur \<rightarrow>\<^sub>f \<langle>A \<times>\<^sub>r twl_st_heur\<rangle> nres_rel\<close>  (is \<open>_ \<in> ?A B\<close>)
+proof -
+  obtain f1 f2 where f: \<open>f = (f1, f2)\<close>
+    by (cases f) auto
+  show ?thesis
+    unfolding f
+    apply (simp only: fref_def twl_st_heur'_def nres_rel_def in_pair_collect_simp)
+    apply (intro conjI impI allI)
+    subgoal for x y
+      using assms[of \<open>length (get_clauses_wl_heur x)\<close>,
+        unfolded twl_st_heur'_def nres_rel_def in_pair_collect_simp f,
+        rule_format] unfolding f
+      apply (simp only: fref_def twl_st_heur'_def nres_rel_def in_pair_collect_simp)
+      apply (drule spec[of _ x])
+      apply (drule spec[of _ y])
+      apply simp
+      apply (rule "weaken_\<Down>'"[of _ \<open>A \<times>\<^sub>r twl_st_heur''' (length (get_clauses_wl_heur x))\<close>])
+      apply (fastforce simp: twl_st_heur'_def)+
+      done
+    done
+qed
+
+definition (in -) lit_of_hd_trail_st_heur :: \<open>twl_st_wl_heur \<Rightarrow> nat literal nres\<close> where
+  \<open>lit_of_hd_trail_st_heur S = do {ASSERT (fst (get_trail_wl_heur S) \<noteq> []); RETURN (lit_of_last_trail_pol (get_trail_wl_heur S))}\<close>
+
+lemma lit_of_hd_trail_st_heur_alt_def:
+  \<open>lit_of_hd_trail_st_heur = (\<lambda>(M, N, D, Q, W, vm, \<phi>). do {ASSERT (fst M \<noteq> []); RETURN (lit_of_last_trail_pol M)})\<close>
+  by (auto simp: lit_of_hd_trail_st_heur_def lit_of_hd_trail_def intro!: ext)
 
 end
