Weidenbach_Book/IsaSAT/IsaSAT_Restart_Heuristics_LLVM.thy
@@ -249,12 +249,8 @@ sepref_def get_reductions_count_fast_code
   unfolding get_reduction_count_alt_def isasat_bounded_assn_def
   by sepref
 
-
 sepref_register get_reductions_count
 
-lemma of_nat_snat:
-  \<open>(id,of_nat) \<in> snat_rel' TYPE('a::len2) \<rightarrow> word_rel\<close>
-  by (auto simp: snat_rel_def snat.rel_def in_br_conv snat_eq_unat)
 
 sepref_def GC_required_heur_fast_code
   is \<open>uncurry GC_required_heur\<close>
@@ -288,26 +284,6 @@ sepref_def isasat_replace_annot_in_trail_code
   apply (rewrite at \<open>list_update _ _ _\<close> annot_index_of_atm)
   by sepref
 
-sepref_register mark_garbage_heur2 mark_garbage_heur4
-sepref_def mark_garbage_heur2_code
-  is \<open>uncurry mark_garbage_heur2\<close>
-  :: \<open>[\<lambda>(C, S). mark_garbage_pre (get_clauses_wl_heur S, C) \<and> arena_is_valid_clause_vdom (get_clauses_wl_heur S) C]\<^sub>a
-     sint64_nat_assn\<^sup>k *\<^sub>a isasat_bounded_assn\<^sup>d \<rightarrow> isasat_bounded_assn\<close>
-  supply [[goals_limit=1]]
-  unfolding mark_garbage_heur2_def isasat_bounded_assn_def
-    fold_tuple_optimizations
-  by sepref
-
-sepref_def mark_garbage_heur4_code
-  is \<open>uncurry mark_garbage_heur4\<close>
-  :: \<open>[\<lambda>(C, S). mark_garbage_pre (get_clauses_wl_heur S, C) \<and> arena_is_valid_clause_vdom (get_clauses_wl_heur S) C \<and>
-        learned_clss_count S \<le> uint64_max]\<^sub>a
-     sint64_nat_assn\<^sup>k *\<^sub>a isasat_bounded_assn\<^sup>d \<rightarrow> isasat_bounded_assn\<close>
-  supply [[goals_limit=1]] isasat_fast_countD[dest] learned_clss_count_def[simp]
-  unfolding mark_garbage_heur4_def isasat_bounded_assn_def
-    fold_tuple_optimizations
-  by sepref
-
 sepref_register remove_one_annot_true_clause_one_imp_wl_D_heur
 
 lemma remove_one_annot_true_clause_one_imp_wl_D_heurI:
@@ -328,17 +304,7 @@ sepref_def remove_one_annot_true_clause_one_imp_wl_D_heur_code
   apply (annot_snat_const \<open>TYPE(64)\<close>)
   by sepref
 
-sepref_register mark_clauses_as_unused_wl_D_heur
-
-sepref_def access_vdom_at_fast_code
-  is \<open>uncurry (RETURN oo access_vdom_at)\<close>
-  :: \<open>[uncurry access_vdom_at_pre]\<^sub>a isasat_bounded_assn\<^sup>k *\<^sub>a sint64_nat_assn\<^sup>k \<rightarrow> sint64_nat_assn\<close>
-  unfolding access_vdom_at_alt_def access_vdom_at_pre_def isasat_bounded_assn_def
-  supply [[goals_limit = 1]]
-  by sepref
-
-
-sepref_register remove_one_annot_true_clause_imp_wl_D_heur
+sepref_register mark_clauses_as_unused_wl_D_heur remove_one_annot_true_clause_imp_wl_D_heur
 
 lemma remove_one_annot_true_clause_imp_wl_D_heurI:
   \<open>learned_clss_count x \<le> uint64_max \<Longrightarrow>
@@ -356,9 +322,6 @@ sepref_def remove_one_annot_true_clause_imp_wl_D_heur_code
   apply (rewrite at \<open>(\<hole>, _)\<close> annot_unat_snat_upcast[where 'l=64])
   apply (annot_unat_const \<open>TYPE(32)\<close>)
   by sepref
-
-(*TODO Move*)
-
 
 
 sepref_def mark_clauses_as_unused_wl_D_heur_fast_code
