Weidenbach_Book/IsaSAT/IsaSAT_Show_LLVM.thy
@@ -1,7 +1,7 @@
 theory IsaSAT_Show_LLVM
   imports
     IsaSAT_Show
-    IsaSAT_Setup_LLVM
+    IsaSAT_Setup0_LLVM
 begin
 
 
