Weidenbach_Book/IsaSAT/IsaSAT_Trail_LLVM.thy
@@ -281,7 +281,7 @@ sepref_def get_the_propagation_reason_fast_code
 
 schematic_goal mk_free_trail_pol_fast_assn[sepref_frame_free_rules]: \<open>MK_FREE trail_pol_fast_assn ?fr\<close>
   unfolding trail_pol_fast_assn_def
-  by (rule free_thms sepref_frame_free_rules)+ (* TODO: Write a method for that! *)
+  by synthesize_free
 
 (*TODO Move*)
 
